cfrontend/Csem.v
@@ -314,12 +314,13 @@ Inductive rred: expr -> mem -> trace -> expr -> mem -> Prop :=
       sem_cast v1 ty1 ty2 m = Some v ->
       rred (Eparen (Eval v1 ty1) ty2 ty) m
         E0 (Eval v ty) m
-  | red_builtin: forall ef tyargs el ty m vargs t vres m',
+  | red_builtin: forall ef tyargs el ty m vargs t vres m' m'',
       cast_arguments m el tyargs vargs ->
-      external_call ef ge vargs m t vres m' ->
+      external_call ef ge vargs (Mem.push_new_stage m) t vres m' ->
+      Mem.unrecord_stack_block m' = Some m'' ->
       forall BUILTIN_ENABLED: builtin_enabled ef,
       rred (Ebuiltin ef tyargs el ty) m
-         t (Eval vres ty) m'.
+         t (Eval vres ty) m''.
 
 
 (** Head reduction for function calls.
@@ -608,7 +609,7 @@ Inductive estep: state -> trace -> state -> Prop :=
       callred a m fd vargs ty i ->
       context RV RV C ->
       estep (ExprState f (C a) k e m)
-         E0 (Callstate fd vargs (Kcall f e C ty k) m (fn_stack_requirements i))
+         E0 (Callstate fd vargs (Kcall f e C ty k) (Mem.push_new_stage m) (fn_stack_requirements i))
 
   | step_stuck: forall C f a k e m K,
       context K RV C -> ~(imm_safe e K a m) ->
@@ -709,26 +710,23 @@ Inductive sstep: state -> trace -> state -> Prop :=
       sstep (State f Sskip (Kfor4 a2 a3 s k) e m)
          E0 (State f (Sfor Sskip a2 a3 s) k e m)
 
-  | step_return_0: forall f k e m m' m'',
+  | step_return_0: forall f k e m m',
       Mem.free_list m (blocks_of_env e) = Some m' ->
-      Mem.unrecord_stack_block m' = Some m'' ->
       sstep (State f (Sreturn None) k e m)
-         E0 (Returnstate Vundef (call_cont k) m'')
+         E0 (Returnstate Vundef (call_cont k) m')
   | step_return_1: forall f x k e m,
       sstep (State f (Sreturn (Some x)) k e m)
          E0 (ExprState f x (Kreturn k) e  m)
-  | step_return_2:  forall f v1 ty k e m v2 m' m'',
+  | step_return_2:  forall f v1 ty k e m v2 m',
       sem_cast v1 ty f.(fn_return) m = Some v2 ->
       Mem.free_list m (blocks_of_env e) = Some m' ->
-      Mem.unrecord_stack_block m' = Some m'' ->
       sstep (ExprState f (Eval v1 ty) (Kreturn k) e m)
-         E0 (Returnstate v2 (call_cont k) m'')
-  | step_skip_call: forall f k e m m' m'',
+         E0 (Returnstate v2 (call_cont k) m')
+  | step_skip_call: forall f k e m m',
       is_call_cont k ->
       Mem.free_list m (blocks_of_env e) = Some m' ->
-      Mem.unrecord_stack_block m' = Some m'' ->
       sstep (State f Sskip k e m)
-         E0 (Returnstate Vundef k m'')
+         E0 (Returnstate Vundef k m')
 
   | step_switch: forall f x sl k e m,
       sstep (State f (Sswitch x sl) k e m)
@@ -759,7 +757,7 @@ Inductive sstep: state -> trace -> state -> Prop :=
       alloc_variables empty_env m (f.(fn_params) ++ f.(fn_vars)) e m1 ->
       frame_adt_blocks fa = blocks_with_info e ->
       frame_adt_size fa = Z.max 0 sz ->
-      Mem.record_stack_blocks (Mem.push_new_stage m1) fa = Some m1' ->
+      Mem.record_stack_blocks m1 fa = Some m1' ->
       bind_parameters e m1' f.(fn_params) vargs m2 ->
       sstep (Callstate (Internal f) vargs k m sz)
          E0 (State f f.(fn_body) k e m2)
@@ -769,9 +767,10 @@ Inductive sstep: state -> trace -> state -> Prop :=
       sstep (Callstate (External ef targs tres cc) vargs k m sz)
           t (Returnstate vres k m')
 
-  | step_returnstate: forall v f e C ty k m,
+  | step_returnstate: forall v f e C ty k m m',
+      Mem.unrecord_stack_block m = Some m' ->
       sstep (Returnstate v (Kcall f e C ty k) m)
-         E0 (ExprState f (C (Eval v ty)) k e m).
+         E0 (ExprState f (C (Eval v ty)) k e m').
 
 Definition step (S: state) (t: trace) (S': state) : Prop :=
   estep S t S' \/ sstep S t S'.
@@ -794,7 +793,7 @@ Inductive initial_state (p: program): state -> Prop :=
       type_of_fundef f = Tfunction Tnil type_int32s cc_default ->
       Mem.alloc m0 0 0 = (m1,b1) ->
       Mem.record_stack_blocks (Mem.push_new_stage m1) (make_singleton_frame_adt b1 0 0) = Some m2 ->
-      initial_state p (Callstate f nil Kstop m2 (fn_stack_requirements (prog_main p))).
+      initial_state p (Callstate f nil Kstop (Mem.push_new_stage m2) (fn_stack_requirements (prog_main p))).
 
 (** A final state is a [Returnstate] with an empty continuation. *)
 
